Continue factoring out facts about solutions and vectors.

Solve.v
@@ -1,3 +1,5 @@
+Require Import Coq.Program.Equality.
+
 Require Import KA.Terms.
 Require Import KA.Vectors.
 Require Import KA.Scope.
@@ -18,7 +20,7 @@ End System.
 Arguments smat {A} {Q}.
 Arguments svec {A} {Q}.
 
-Section Solve.
+Section SolutionDefinition.
   Context {A: Type}.
   Notation term := (term A).
   Notation matrix := (matrix A).
@@ -53,6 +55,23 @@ Section Solve.
       sol <== sol'
   }.
 
+  Definition solution_nat
+    {n: nat}
+    (sys: system (position n))
+    (scale: term)
+    (sol: vector (position n))
+  :=
+    smat sys <*> sol <+> svec sys ;;; scale <== sol
+  .
+End SolutionDefinition.
+
+Section SolutionAlgorithm.
+  Context {A: Type}.
+  Notation term := (term A).
+  Notation matrix := (matrix A).
+  Notation vector := (vector A).
+  Notation system := (system A).
+
   Definition compress_system
     {n: nat}
     (sys: system (position (S n)))
@@ -84,4 +103,289 @@ Section Solve.
       (smat sys PHere PHere)* ;;
         (svec sys PHere + (# (smat sys PHere)) ** smaller_solution);
   }.
-End Solve.
+End SolutionAlgorithm.
+
+Section SolutionCorrect.
+  Context {A: Type}.
+  Notation term := (term A).
+  Notation matrix := (matrix A).
+  Notation vector := (vector A).
+  Notation system := (system A).
+
+  Lemma compute_solution_nat_chomp
+    {n: nat}
+    (sys: system (position (S n)))
+  :
+    # compute_solution_nat sys === compute_solution_nat (compress_system sys)
+  .
+  Proof.
+    intro.
+    unfold vector_chomp.
+    now autorewrite with compute_solution_nat; simpl.
+  Qed.
+
+  Lemma compress_system_mat
+    (n: nat)
+    (sys: system (position (S n)))
+    (p: position n)
+  :
+    (smat sys (PThere p) PHere;; smat sys PHere PHere *) &
+      (# smat sys PHere) <+> # smat sys (PThere p)
+    === smat (compress_system sys) p
+  .
+  Proof.
+    unfold compress_system; simpl.
+    intro.
+    unfold vector_sum, vector_scale_left, vector_chomp.
+    now rewrite EPlusComm.
+  Qed.
+
+  Lemma compress_system_vec
+    (n: nat)
+    (sys: system (position (S n)))
+    (p: position n)
+  :
+    svec sys (PThere p) +
+      smat sys (PThere p) PHere ;; smat sys PHere PHere * ;; svec sys PHere
+    == svec (compress_system sys) p
+  .
+  Proof.
+    now unfold compress_system; simpl.
+  Qed.
+
+  Lemma solution_iff_solution_nat
+    {n: nat}
+    (sys: system (position n))
+    (scale: term)
+    (sol: vector (position n))
+  :
+    solution sys scale sol <-> solution_nat sys scale sol
+  .
+  Proof.
+    split; intros.
+    - unfold solution_nat.
+      intro p.
+      unfold vector_sum, matrix_vector_product.
+      apply term_lequiv_split.
+      + apply vector_inner_product_contained_split; intro.
+        apply H.
+      + apply H.
+    - split; intros.
+      + eapply term_lequiv_trans; [apply term_lequiv_split_left|].
+        * apply vector_inner_product_contained.
+        * apply H.
+      + eapply term_lequiv_trans; [apply term_lequiv_split_right|].
+        * apply term_lequiv_refl.
+        * apply H.
+  Qed.
+
+  Lemma solution_one_solution_nat
+    {Q: Type}
+    (sys: system Q)
+    (scale: term)
+    (sol: vector Q)
+  :
+    solution sys 1 sol ->
+    solution sys scale (sol ;;; scale)
+  .
+  Proof.
+    split; intros.
+    - unfold vector_scale_right.
+      rewrite ETimesAssoc.
+      apply times_mor_mono; try reflexivity.
+      apply H.
+    - unfold vector_scale_right.
+      apply times_mor_mono; try reflexivity.
+      unfold term_lequiv.
+      rewrite <- ETimesUnitRight with (t := svec sys q).
+      apply H.
+  Qed.
+
+  Lemma compute_solution_nat_solution_nat_one
+    {n: nat}
+    (sys: system (position n))
+  :
+    solution_nat sys 1 (compute_solution_nat sys)
+  .
+  Proof.
+    unfold solution_nat; intro p.
+    dependent induction p.
+    + unfold vector_sum, matrix_vector_product.
+      autorewrite with inner_product.
+      autorewrite with compute_solution_nat; simpl.
+      rewrite ETimesAssoc.
+      unfold vector_scale_right; rewrite ETimesUnitRight.
+      rewrite <- EPlusAssoc with (t3 := svec sys PHere).
+      rewrite EPlusComm with (t2 := svec sys PHere).
+      rewrite <- ETimesUnitLeft
+        with (t := _ + # _ ** # compute_solution_nat sys).
+      rewrite compute_solution_nat_chomp.
+      rewrite <- EDistributeRight.
+      rewrite <- EStarLeft.
+      apply term_lequiv_refl.
+    + unfold vector_sum, matrix_vector_product.
+      autorewrite with inner_product.
+      autorewrite with compute_solution_nat; simpl.
+      rewrite ETimesAssoc.
+      rewrite EDistributeLeft.
+      rewrite compute_solution_nat_chomp.
+      rewrite vector_inner_product_scale_left.
+      rewrite <- EPlusAssoc with (t1 := _ ;; svec sys PHere).
+      rewrite vector_inner_product_distribute_left.
+      rewrite compress_system_mat.
+      rewrite EPlusComm with (t1 := _ ;; svec sys PHere).
+      unfold vector_scale_right; rewrite ETimesUnitRight.
+      rewrite <- EPlusAssoc with (t3 := svec sys (PThere p)).
+      rewrite EPlusComm with (t2 := svec sys (PThere p)) .
+      rewrite compress_system_vec.
+      unfold vector_scale_right, vector_sum in IHp;
+      setoid_rewrite ETimesUnitRight in IHp.
+      apply IHp.
+  Qed.
+
+  Lemma solution_bound_mat
+    {Q: Type}
+    (sys: system Q)
+    (scale: term)
+    (sol: vector Q)
+    (q q': Q)
+  :
+    solution sys scale sol ->
+    term_lequiv ((smat sys q q)* ;; smat sys q q' ;; sol q') (sol q)
+  .
+  Proof.
+    intros.
+    rewrite <- ETimesAssoc.
+    apply EFixLeft.
+    apply term_lequiv_split;
+    apply H.
+  Qed.
+
+  Lemma solution_bound_vec
+    {Q: Type}
+    (sys: system Q)
+    (scale: term)
+    (sol: vector Q)
+    (q: Q)
+  :
+    solution sys scale sol ->
+    term_lequiv ((smat sys q q)* ;; svec sys q ;; scale) (sol q)
+  .
+  Proof.
+    intros.
+    rewrite <- ETimesAssoc.
+    apply EFixLeft.
+    apply term_lequiv_split;
+    apply H.
+  Qed.
+
+  Lemma solution_bound
+    {Q: Type}
+    (sys: system Q)
+    (scale: term)
+    (sol: vector Q)
+    (q q': Q)
+  :
+    solution sys scale sol ->
+    term_lequiv ((smat sys q q)* ;; (smat sys q q' ;; sol q' + svec sys q ;; scale)) (sol q)
+  .
+  Proof.
+    intros.
+    rewrite EDistributeLeft.
+    apply term_lequiv_split.
+    + rewrite ETimesAssoc.
+      eapply solution_bound_mat; eauto.
+    + rewrite ETimesAssoc.
+      now apply solution_bound_vec.
+  Qed.
+
+  Lemma solution_project
+    {n: nat}
+    (sys: system (position (S n)))
+    (scale: term)
+    (sol: vector (position (S n)))
+  :
+    solution sys scale sol ->
+    solution (compress_system sys) scale (# sol)
+  .
+  Proof.
+    split; intros; simpl;
+    rewrite EDistributeRight;
+    unfold vector_chomp.
+    - apply term_lequiv_split.
+      + apply H.
+      + fold_term_lequiv.
+        repeat rewrite <- ETimesAssoc.
+        rewrite ETimesAssoc with (t3 := sol (PThere q')).
+        erewrite solution_bound_mat; eauto.
+        apply H.
+    - apply term_lequiv_split.
+      + apply H.
+      + fold_term_lequiv.
+        repeat rewrite <- ETimesAssoc.
+        rewrite ETimesAssoc with (t3 := scale).
+        erewrite solution_bound_vec; eauto.
+        apply H.
+  Qed.
+
+  Lemma compute_solution_nat_least
+    {n: nat}
+    (sys: system (position n))
+    (scale: term)
+    (sol: vector (position n))
+  :
+    solution_nat sys scale sol ->
+    compute_solution_nat sys ;;; scale <== sol
+  .
+  Proof.
+    intros.
+    dependent induction n; intro p; dependent destruction p.
+    - unfold vector_scale_right.
+      autorewrite with compute_solution_nat; simpl.
+      rewrite EPlusComm with (t1 := svec sys PHere).
+      fold_term_lequiv.
+      rewrite <- ETimesAssoc.
+      rewrite EDistributeRight.
+      rewrite vector_inner_product_scale_right.
+      rewrite IHn with (sol := # sol).
+      + rewrite EDistributeLeft.
+        apply term_lequiv_split.
+        * rewrite vector_inner_product_scale_left.
+          apply vector_inner_product_contained_split; intros.
+          unfold vector_scale_left.
+          unfold vector_chomp.
+          eapply solution_bound_mat.
+          now apply solution_iff_solution_nat.
+        * rewrite ETimesAssoc.
+          apply solution_bound_vec.
+          now apply solution_iff_solution_nat.
+      + apply solution_iff_solution_nat.
+        apply solution_project.
+        now apply solution_iff_solution_nat.
+    - autorewrite with compute_solution_nat; simpl.
+      eapply term_lequiv_trans; swap 1 2.
+      apply (IHn (compress_system sys) scale (# sol)).
+      + apply solution_iff_solution_nat.
+        apply solution_project.
+        now apply solution_iff_solution_nat.
+      + unfold vector_scale_right.
+        autorewrite with compute_solution_nat; simpl.
+        apply term_lequiv_refl.
+  Qed.
+
+  Lemma compute_solution_nat_least_solution
+    {n: nat}
+    (sys: system (position n))
+    (scale: term)
+  :
+    least_solution sys scale (compute_solution_nat sys ;;; scale)
+  .
+  Proof.
+    split.
+    - apply solution_one_solution_nat.
+      apply solution_iff_solution_nat.
+      apply compute_solution_nat_solution_nat_one.
+    - setoid_rewrite solution_iff_solution_nat.
+      apply compute_solution_nat_least.
+  Qed.
+End SolutionCorrect.
