Vectors.v
@@ -63,13 +63,32 @@ Section VectorOperations.
   :=
     inner_product (m p) v
   .
-End VectorOperations.
 
+  Definition vector_scale_left
+    {Q: Type}
+    (t: term)
+    (v: vector Q)
+    (q: Q)
+  :=
+    t ;; v q
+  .
+
+  Definition vector_scale_right
+    {Q: Type}
+    (v: vector Q)
+    (t: term)
+    (q: Q)
+  :=
+    v q ;; t
+  .
+End VectorOperations.
 
 Notation "v1 <+> v2" := (vector_sum v1 v2) (at level 40) : ka_scope.
 Notation "# v" := (vector_chomp v) (at level 30) : ka_scope.
 Notation "v1 ** v2" := (inner_product v1 v2) (at level 40) : ka_scope.
 Notation "m <*> v" := (matrix_vector_product m v) (at level 40) : ka_scope.
+Notation "t & v" := (vector_scale_left t v) (at level 30) : ka_scope.
+Notation "v ;;; t" := (vector_scale_right v t) (at level 35) : ka_scope.
 
 Section VectorEquiv.
   Context {A: Type}.
@@ -155,3 +174,178 @@ End VectorEquiv.
 
 Notation "v1 === v2" := (equiv_vec v1 v2) (at level 70) : ka_scope.
 Notation "v1 <== v2" := (lequiv_vec v1 v2) (at level 70) : ka_scope.
+
+Section VectorProperties.
+  Context {A: Type}.
+  Notation term := (term A).
+  Notation vector := (vector A).
+
+  Lemma vector_scale_left_chomp
+    {n: nat}
+    (t: term)
+    (v: vector (position (S n)))
+  :
+    t & (# v) === # (t & v)
+  .
+  Proof.
+    now intro.
+  Qed.
+
+  Lemma vector_inner_product_scale_left
+    {n: nat}
+    (t: term)
+    (v1 v2: vector (position n))
+  :
+    t ;; (v1 ** v2) == (t & v1) ** v2
+  .
+  Proof.
+    dependent induction n.
+    - autorewrite with inner_product.
+      now rewrite ETimesZeroLeft.
+    - autorewrite with inner_product.
+      rewrite EDistributeLeft.
+      rewrite IHn.
+      unfold vector_scale_left at 2; simpl.
+      rewrite vector_scale_left_chomp.
+      rewrite ETimesAssoc.
+      reflexivity.
+  Qed.
+
+  Lemma vector_chomp_sum
+    {n: nat}
+    (v1 v2: vector (position (S n)))
+  :
+    # (v1 <+> v2) === # v1 <+> # v2
+  .
+  Proof.
+    now intro.
+  Qed.
+
+  Lemma vector_inner_product_distribute_left
+    {n: nat}
+    (v1 v2 v3: vector (position n))
+  :
+    v1 ** v3 + v2 ** v3 == (v1 <+> v2) ** v3
+  .
+  Proof.
+    dependent induction n.
+    - autorewrite with inner_product.
+      now rewrite EPlusIdemp.
+    - autorewrite with inner_product.
+      rewrite EPlusAssoc.
+      rewrite <- EPlusAssoc with (t3 := v2 PHere ;; v3 PHere).
+      rewrite EPlusComm with (t1 := # v1 ** # v3).
+      rewrite EPlusAssoc.
+      rewrite <- EDistributeRight.
+      rewrite <- EPlusAssoc.
+      rewrite IHn.
+      unfold vector_sum at 2.
+      rewrite vector_chomp_sum.
+      reflexivity.
+  Qed.
+
+  Lemma vector_inner_product_contained
+    {n: nat}
+    (v1 v2: vector (position n))
+    (p: position n)
+  :
+    v1 p ;; v2 p <= v1 ** v2
+  .
+  Proof.
+    dependent induction p.
+    - autorewrite with inner_product.
+      apply term_lequiv_split_left.
+      apply term_lequiv_refl.
+    - autorewrite with inner_product.
+      apply term_lequiv_split_right.
+      fold ((# v1) p).
+      fold ((# v2) p).
+      apply IHp.
+  Qed.
+
+  Global Add Parametric Morphism (n: nat): inner_product
+    with signature eq ==> (@lequiv_vec A (position n)) ==> term_lequiv
+    as inner_product_mor_mono
+  .
+  Proof.
+    unfold term_lequiv; intros.
+    dependent induction n.
+    - autorewrite with inner_product.
+      apply term_lequiv_refl.
+    - autorewrite with inner_product.
+      apply term_lequiv_split.
+      + rewrite <- (H PHere).
+        rewrite EDistributeLeft.
+        repeat apply term_lequiv_split_left.
+        apply term_lequiv_refl.
+      + apply term_lequiv_split_right.
+        apply IHn.
+        intro p.
+        apply H.
+  Qed.
+
+  Lemma vector_inner_product_contained_split
+    {n: nat}
+    (v1 v2: vector (position n))
+    (t: term)
+  :
+    (forall p, v1 p ;; v2 p <= t) ->
+    v1 ** v2 <= t
+  .
+  Proof.
+    intros.
+    dependent induction n.
+    - autorewrite with inner_product.
+      rewrite EPlusComm.
+      now rewrite EPlusUnit.
+    - autorewrite with inner_product.
+      apply term_lequiv_split.
+      + apply H.
+      + apply IHn; intros.
+        unfold vector_chomp.
+        apply H.
+  Qed.
+
+  Lemma vector_scale_right_unit
+    {Q: Type}
+    (v: vector Q)
+  :
+    v ;;; 1 === v
+  .
+  Proof.
+    intro q.
+    unfold vector_scale_right.
+    now rewrite ETimesUnitRight.
+  Qed.
+
+  Lemma vector_scale_right_chomp
+    {n: nat}
+    (v: vector (position (S n)))
+    (t: term)
+  :
+    (# v) ;;; t === # (v ;;; t)
+  .
+  Proof.
+    now intro.
+  Qed.
+
+  Lemma vector_inner_product_scale_right
+    {n: nat}
+    (v1 v2: vector (position n))
+    (t: term)
+  :
+    (v1 ** v2) ;; t == v1 ** (v2 ;;; t)
+  .
+  Proof.
+    dependent induction n.
+    - autorewrite with inner_product.
+      now rewrite ETimesZeroRight.
+    - autorewrite with inner_product.
+      rewrite EDistributeRight.
+      rewrite IHn.
+      unfold vector_scale_right at 2; simpl.
+      rewrite vector_scale_right_chomp.
+      rewrite ETimesAssoc.
+      reflexivity.
+  Qed.
+  End VectorProperties.
